Updates

intermediate2/Zeta.Intermediate.Global.fsti
@@ -6,7 +6,9 @@ open Zeta.Intermediate.Verifier
 open Zeta.Intermediate.Logs
 open Zeta.Generic.Global
 
+module S = FStar.Seq
 module IT = Zeta.Intermediate.Thread
+module HG = Zeta.High.Global
 
 let verifiable_log (vcfg:_)
   = Zeta.Generic.Global.verifiable_log (int_verifier_spec vcfg)
@@ -20,3 +22,9 @@ let to_logk_entry (#vcfg:_) (gl: verifiable_log vcfg) (i: sseq_index gl)
     let tl = index gl t in
     IT.to_logk_entry tl j
 
+let global_rel (#vcfg:_) (gl: verifiable_log vcfg) (glk: HG.verifiable_log vcfg.app)
+  = S.length gl = S.length glk /\
+    (forall t. IT.thread_rel (index gl t) (index glk t))
+
+val global_rel_implies_appfn_identical (#vcfg:_) (gls: verifiable_log vcfg) (glk: _{global_rel gls glk})
+  : Lemma (ensures (app_fcrs gls = app_fcrs glk))
